Proofs for pre-fancy pass (could use cleanup)

src/Experiments/SimplyTypedArithmetic.v
@@ -3031,14 +3031,14 @@ Module Compilers.
                  | Z_mul_split => curry3 Z.mul_split
                  | Z_mul_split_concrete s => curry2 (Z.mul_split s)
                  | Z_add_get_carry => curry3 Z.add_get_carry_full
-                 | Z_add_get_carry_concrete s => curry2 (Z.add_get_carry s)
+                 | Z_add_get_carry_concrete s => curry2 (Z.add_get_carry_full s)
                  | Z_add_with_carry => curry3 Z.add_with_carry
                  | Z_add_with_get_carry => curry4 Z.add_with_get_carry_full
-                 | Z_add_with_get_carry_concrete s => curry3 (Z.add_with_get_carry s)
+                 | Z_add_with_get_carry_concrete s => curry3 (Z.add_with_get_carry_full s)
                  | Z_sub_get_borrow => curry3 Z.sub_get_borrow_full
-                 | Z_sub_get_borrow_concrete s => curry2 (Z.sub_get_borrow s)
+                 | Z_sub_get_borrow_concrete s => curry2 (Z.sub_get_borrow_full s)
                  | Z_sub_with_get_borrow => curry4 Z.sub_with_get_borrow_full
-                 | Z_sub_with_get_borrow_concrete s => curry3 (Z.sub_with_get_borrow s)
+                 | Z_sub_with_get_borrow_concrete s => curry3 (Z.sub_with_get_borrow_full s)
                  | Z_zselect => curry3 Z.zselect
                  | Z_add_modulo => curry3 Z.add_modulo
                  | Z_rshi => curry4 Z.rshi
@@ -4198,13 +4198,13 @@ Module Compilers.
                   | ident.Z_mul_split_concrete s
                     => cps_of (curry2 (Z.mul_split s))
                   | ident.Z_add_get_carry_concrete s
-                    => cps_of (curry2 (Z.add_get_carry s))
+                    => cps_of (curry2 (Z.add_get_carry_full s))
                   | ident.Z_add_with_get_carry_concrete s
-                    => cps_of (curry3 (Z.add_with_get_carry s))
+                    => cps_of (curry3 (Z.add_with_get_carry_full s))
                   | ident.Z_sub_get_borrow_concrete s
-                    => cps_of (curry2 (Z.sub_get_borrow s))
+                    => cps_of (curry2 (Z.sub_get_borrow_full s))
                   | ident.Z_sub_with_get_borrow_concrete s
-                    => cps_of (curry3 (Z.sub_with_get_borrow s))
+                    => cps_of (curry3 (Z.sub_with_get_borrow_full s))
                   | ident.Z_rshi_concrete s n
                     => cps_of (curry2 (fun x y => Z.rshi s x y n))
                   | ident.Z_cc_m_concrete s
@@ -7919,6 +7919,22 @@ End X25519_32.
 
 Module Straightline.
   Module expr.
+    (* TODO: move these to a better location *)
+    Module type.
+      Definition primitive_eq_dec (a b : type.primitive) : {a = b} + {a <> b}.
+      Proof. destruct a,b; auto; right; congruence. Defined.
+      Fixpoint type_eq_dec (a b : type) : {a = b} + {a <> b}.
+      Proof.
+        destruct a, b; try solve [right; congruence]; [ | | | ].
+        { destruct (primitive_eq_dec p p0); subst; [left | right]; congruence. }
+        { destruct (type_eq_dec a1 b1); destruct (type_eq_dec a2 b2); subst; try solve [right; congruence].
+          left; congruence. }
+        { destruct (type_eq_dec a1 b1); destruct (type_eq_dec a2 b2); subst; try solve [right; congruence].
+          left; congruence. }
+        { destruct (type_eq_dec a b); [left | right]; congruence. }
+      Defined.
+    End type.
+
     Section with_var.
       Context {var : type.type -> Type}.
       Context {dummy_arrow : forall s d, var (s -> d)}. (* TODO: remove once arrow-containing pairs are removed at type level *)
@@ -7927,24 +7943,26 @@ Module Straightline.
 
       Section with_ident.
         Context {ident : type.type -> type.type -> Type}.
+        Inductive scalar : type.type -> Type :=
+        | Var t : var t -> scalar t
+        | TT : scalar (type.type_primitive type.unit)
+        | Nil t : scalar (type.list t)
+        | Pair {a b} : scalar a -> scalar b -> scalar (a * b)
+        | Cast : zrange -> scalar type.Z -> scalar type.Z
+        | Cast2 : zrange * zrange -> scalar (type.Z*type.Z) -> scalar (type.Z*type.Z)
+        | Fst {a b} : scalar (a * b) -> scalar a
+        | Snd {a b} : scalar (a * b) -> scalar b
+        | Shiftr : Z -> scalar type.Z -> scalar type.Z
+        | Shiftl : Z -> scalar type.Z -> scalar type.Z
+        | Land : Z -> scalar type.Z -> scalar type.Z
+        | CC_m : Z -> scalar type.Z -> scalar type.Z
+        | Primitive {t} : type.interp (type.type_primitive t) -> scalar t
+        .
+
         Inductive expr : type.type -> Type :=
         | Scalar {t} : scalar t -> expr t
         | LetInAppIdentZ {s d} : zrange -> ident s (type.Z) -> scalar s -> (var (type.Z) -> expr d) -> expr d
         | LetInAppIdentZZ {s d} : zrange * zrange -> ident s (type.Z*type.Z) -> scalar s -> (var (type.Z*type.Z) -> expr d) -> expr d
-        with scalar : type.type -> Type :=
-             | Var t : var t -> scalar t
-             | TT : scalar (type.type_primitive type.unit)
-             | Nil t : scalar (type.list t)
-             | Pair {a b} : scalar a -> scalar b -> scalar (a * b)
-             | Cast : zrange -> scalar type.Z -> scalar type.Z
-             | Cast2 : zrange * zrange -> scalar (type.Z*type.Z) -> scalar (type.Z*type.Z)
-             | Fst {a b} : scalar (a * b) -> scalar a
-             | Snd {a b} : scalar (a * b) -> scalar b
-             | Shiftr : Z -> scalar type.Z -> scalar type.Z
-             | Shiftl : Z -> scalar type.Z -> scalar type.Z
-             | Land : Z -> scalar type.Z -> scalar type.Z
-             | CC_m : Z -> scalar type.Z -> scalar type.Z
-             | Primitive {t} : type.interp (type.type_primitive t) -> scalar t
         .
 
         Fixpoint dummy_scalar t : scalar t :=
@@ -7960,7 +7978,7 @@ Module Straightline.
 
       Definition of_uncurried_scalar_ident {s d} (idc : ident.ident s d)
         : scalar s -> option (scalar d) :=
-        match idc in ident.ident s d return scalar (ident:=ident.ident) s -> option (scalar d) with
+        match idc in ident.ident s d return scalar s -> option (scalar d) with
         | ident.Z.cast r => fun args => Some (Cast r args)
         | ident.Z.cast2 r => fun args => Some (Cast2 r args)
         | @ident.fst A B => fun args => Some (Fst args)
@@ -8131,20 +8149,20 @@ Module Straightline.
     End depth.
 
     Section interp.
-      Local Notation scalar := (@scalar type.interp default.ident).
-      Local Notation expr := (@expr type.interp default.ident).
+      Context {ident : type -> type -> Type} {interp_ident : forall s d, ident s d -> type.interp s -> type.interp d}.
 
       Definition interp_cast (r : zrange) (x : Z) : Z := ident.cast ident.cast_outside_of_range r x.
-      
-      Fixpoint interp_scalar {t} (s : scalar t) : type.interp t :=
+      Definition interp_cast2 (r : zrange * zrange) (x : Z * Z) : Z * Z :=
+        (interp_cast (fst r) (fst x), interp_cast (snd r) (snd x)).
+
+      Fixpoint interp_scalar {t} (s : @scalar type.interp t) : type.interp t :=
         match s with
         | Var t v => v
         | TT => tt
         | Nil _ => []
         | Pair _ _ x y => (interp_scalar x, interp_scalar y)
         | Cast r x => interp_cast r (interp_scalar x)
-        | Cast2 r x =>
-          let '(a,b) := interp_scalar x in (interp_cast (fst r) a, interp_cast (snd r) b)
+        | Cast2 r x => interp_cast2 r (interp_scalar x)
         | Fst _ _ p => fst (interp_scalar p)
         | Snd _ _ p => snd (interp_scalar p)
         | Shiftr n x => Z.shiftr (interp_scalar x) n
@@ -8154,15 +8172,20 @@ Module Straightline.
         | Primitive _ x => x
         end.
       
-      Fixpoint interp {t} (e : expr t) : type.interp t :=
+      Fixpoint interp {t} (e : @expr type.interp ident t) : type.interp t :=
         match e with
         | Scalar _ s => interp_scalar s
         | LetInAppIdentZ _ _ r idc x f =>
-          interp (f (interp_cast r (ident.interp idc (interp_scalar x))))
-        | LetInAppIdentZZ _ _ (r1,r2) idc x f =>
-          let '(a,b) := ident.interp idc (interp_scalar x) in
-          interp (f (interp_cast r1 a, interp_cast r2 b))
+          interp (f (interp_cast r (interp_ident _ _ idc (interp_scalar x))))
+        | LetInAppIdentZZ _ _ r idc x f =>
+          interp (f (interp_cast2 r (interp_ident _ _ idc (interp_scalar x))))
         end.
+    End interp.
+
+    Section proofs.
+      Local Notation straightline_interp := (expr.interp (ident:=default.ident) (interp_ident:=@ident.interp)).
+      Local Notation uinterp := (Uncurried.expr.interp (@ident.interp)).
+      Local Notation uexpr := (@Uncurried.expr.expr ident type.interp).
 
       Inductive ok_scalar_ident : forall {s d}, ident.ident s d -> Prop :=
       | ok_si_cast : forall r, ok_scalar_ident (ident.Z.cast r)
@@ -8176,7 +8199,7 @@ Module Straightline.
       | ok_prim : forall p x, ok_scalar_ident (@ident.primitive p x)
       .
 
-      Inductive ok_scalar: forall {t}, @Uncurried.expr.expr ident type.interp t -> Prop :=
+      Inductive ok_scalar: forall {t}, uexpr t -> Prop :=
       | ok_Var : forall t v, @ok_scalar t (Uncurried.expr.Var v)
       | ok_TT : ok_scalar Uncurried.expr.TT
       | ok_AppIdent :
@@ -8191,7 +8214,7 @@ Module Straightline.
             ok_scalar (Uncurried.expr.Pair a b)
       .
 
-      Inductive ok_expr : forall {t}, Uncurried.expr.expr t -> Prop :=
+      Inductive ok_expr : forall {t}, uexpr t -> Prop :=
       | ok_LetInAppIdentZ :
           forall tC r s (idc : ident s type.Z) x k,
             ok_scalar x -> (forall y, @ok_expr tC (k y)) ->
@@ -8214,34 +8237,18 @@ Module Straightline.
           forall t x, @ok_scalar t x -> @ok_expr t x
       .
 
-      Lemma interp_cast_correct {t} r (idc : ident t type.Z) x :
-        interp_cast r (ident.interp idc (expr.interp (@ident.interp) x))
-        = expr.interp (@ident.interp) (AppIdent (ident.Z.cast r) (AppIdent idc x)).
+      Lemma interp_cast_correct r (x : uexpr type.Z) :
+        interp_cast r (uinterp x) = uinterp (AppIdent (ident.Z.cast r) x).
       Proof. reflexivity. Qed.
 
-      Lemma interp_cast2_correct {t} r1 r2 (idc : ident t (type.prod type.Z type.Z)) x :
-        (interp_cast r1 (fst (ident.interp idc (expr.interp (@ident.interp) x))),
-         interp_cast r2 (snd (ident.interp idc (expr.interp (@ident.interp) x))))
-        = expr.interp (@ident.interp) (AppIdent (ident.Z.cast2 (r1, r2)) (AppIdent idc x)).
+      Lemma interp_cast2_correct r (x : uexpr (type.prod type.Z type.Z)) :
+        interp_cast2 r (uinterp x) = uinterp (AppIdent (ident.Z.cast2 r) x).
       Proof. cbn; break_match; reflexivity. Qed.
-
-      Definition primitive_eq_dec (a b : type.primitive) : {a = b} + {a <> b}.
-      Proof. destruct a,b; auto; right; congruence. Defined.
-      Fixpoint type_eq_dec (a b : type) : {a = b} + {a <> b}.
-      Proof.
-        destruct a, b; try solve [right; congruence]; [ | | | ].
-        { destruct (primitive_eq_dec p p0); subst; [left | right]; congruence. }
-        { destruct (type_eq_dec a1 b1); destruct (type_eq_dec a2 b2); subst; try solve [right; congruence].
-          left; congruence. }
-        { destruct (type_eq_dec a1 b1); destruct (type_eq_dec a2 b2); subst; try solve [right; congruence].
-          left; congruence. }
-        { destruct (type_eq_dec a b); [left | right]; congruence. }
-      Defined.
 
       Ltac invert H :=
         inversion H; subst;
         repeat match goal with
-               | H : existT _ _ _ = existT _ _ _ |- _ => apply (Eqdep_dec.inj_pair2_eq_dec _ type_eq_dec) in H; subst
+               | H : existT _ _ _ = existT _ _ _ |- _ => apply (Eqdep_dec.inj_pair2_eq_dec _ type.type_eq_dec) in H; subst
                end.
 
       Ltac invert_ok_expr :=
@@ -8253,7 +8260,7 @@ Module Straightline.
       Ltac simpl_inversions :=
         cbn [invert_LetInAppIdent invert_LetInCast invert_Pair invert_cast invert_AppIdent invert_Abs].
 
-      Lemma invert_AppIdent_correct {d} (e : @Uncurried.expr.expr ident type.interp d) x p :
+      Lemma invert_AppIdent_correct {d} (e : uexpr d) x p :
         invert_AppIdent e = Some (existT (fun s : type => (ident s d * default.expr s)%type) x p) ->
         e = AppIdent (fst p) (snd p).
       Proof.
@@ -8268,37 +8275,38 @@ Module Straightline.
       Lemma of_uncurried_scalar_ident_correct {s d} (idc : ident s d) args args':
         ok_scalar_ident idc ->
         of_uncurried_scalar args = Some args' ->
-        interp_scalar args' = expr.interp (@ident.interp) args ->
+        interp_scalar args' = uinterp args ->
         exists s,
           of_uncurried_scalar_ident idc args' = Some s
-          /\ interp_scalar s = expr.interp (@ident.interp) (AppIdent idc args).
+          /\ interp_scalar s = uinterp (AppIdent idc args).
       Proof.
         destruct 1; intros;
           repeat match goal with
                  | _ => eexists; split; [ reflexivity | cbn [interp_scalar] ]
                  | H : interp_scalar _ = _ |- _ => rewrite H
                  | _ => reflexivity
+                 | _ => solve [auto using interp_cast2_correct]
+                 | |- context [@Uncurried.expr.interp _ _ (type.type_primitive _)] =>
+                   cbn; break_match; reflexivity
                  end.
-        { cbn; break_match; reflexivity. }
-        { cbn; break_match; reflexivity. }
       Qed.
 
-      Lemma of_uncurried_scalar_correct {t} (e : Uncurried.expr.expr t) :
+      Lemma of_uncurried_scalar_correct {t} (e : uexpr t) :
         ok_scalar e ->
         exists s,
           of_uncurried_scalar e = Some s
-          /\ interp_scalar s = expr.interp (@ident.interp) e.
+          /\ interp_scalar s = uinterp  e.
       Proof.
         induction 1; cbn [of_uncurried_scalar]; intros;
           repeat match goal with
+                 | _ => progress cbn [interp_scalar]
                  | IH : exists _, _ /\ _ |- _ => destruct IH as [? [? ?] ]
                  | H : of_uncurried_scalar _ = _ |- _ => rewrite H
+                 | H : interp_scalar _ = _ |- _ => rewrite H
                  | _ => apply of_uncurried_scalar_ident_correct; solve [auto]
-                 | _ => eexists; tauto
-                 end; [ ].
-        eexists; split; [ reflexivity | ].
-        cbn [interp_scalar expr.interp].
-        congruence.
+                 | _ => eexists; split; [ reflexivity | ]
+                 | _ => reflexivity
+                 end.
       Qed.
 
       Ltac rewrite_ok_scalar :=
@@ -8312,10 +8320,10 @@ Module Straightline.
                end.
       
       Lemma of_uncurried_correct dummy_arrow fuel dummy_var :
-        forall {t} (e : @Uncurried.expr.expr ident type.interp t),
+        forall {t} (e : uexpr t),
         (depth _ dummy_var e <= fuel)%nat ->
         ok_expr e ->
-        expr.interp (@ident.interp) e = interp (@of_uncurried _ dummy_arrow fuel _ e).
+        uinterp e = straightline_interp (@of_uncurried _ dummy_arrow fuel _ e).
       Proof.
         induction fuel; intros; [ pose proof (depth_positive dummy_var e); omega | ].
         destruct e; cbn [depth of_uncurried expr.interp interp]; intros; invert_ok_expr;
@@ -8327,7 +8335,7 @@ Module Straightline.
                  end; [ | | | | ].
         {
           match goal with H : interp_scalar _ = _ |- _ => rewrite H end.
-          rewrite <-IHfuel; rewrite interp_cast_correct.
+          rewrite <-IHfuel.
           { reflexivity. }
           { cbn [depth] in *.
             (* here we have to reason about the depth calculation for arrows; this will probably be unnecessary with new compilers setup *)
@@ -8335,12 +8343,7 @@ Module Straightline.
           { auto. } }
         {
           match goal with H : interp_scalar _ = _ |- _ => rewrite H end.
-          break_match.
-          match goal with H : ?p = (?x, ?y) |- _ =>
-                          replace x with (fst p) by (rewrite H; reflexivity);
-                          replace y with (snd p) by (rewrite H; reflexivity)
-          end.
-          rewrite <-IHfuel. rewrite interp_cast2_correct.
+          rewrite <-IHfuel.
           { cbn; break_match; reflexivity. }
           { cbn [depth] in *.
             (* here we have to reason about the depth calculation for arrows; this will probably be unnecessary with new compilers setup *)
@@ -8348,16 +8351,11 @@ Module Straightline.
           { auto. } }
         {
           match goal with H : interp_scalar _ = _ |- _ => rewrite H end.
-          rewrite interp_cast_correct.
+          rewrite <-interp_cast_correct.
           reflexivity. }
         {
           match goal with H : interp_scalar _ = _ |- _ => rewrite H end.
-          break_match.
-          match goal with H : ?p = (?x, ?y) |- _ =>
-                          replace x with (fst p) by (rewrite H; reflexivity);
-                          replace y with (snd p) by (rewrite H; reflexivity)
-          end.
-          rewrite interp_cast2_correct.
+          rewrite <-interp_cast2_correct.
           cbn; break_match; reflexivity. }
         { invert_ok_scalar.
           rewrite <-H2.
@@ -8385,7 +8383,7 @@ Module Straightline.
             repeat match goal with H : interp_scalar _ = _ |- _ => rewrite H end.
             destruct r; reflexivity. }
         Admitted.
-    End interp.
+    End proofs.
   End expr.
 
   Definition of_Expr {s d} (e : Expr (s->d)) (var : type -> Type) (x:var s) dummy_arrow: expr.expr d
@@ -8466,213 +8464,848 @@ End StraightlineTest.
 
 (* Convert straightline code to code that uses only a certain set of identifiers *)
 Module PreFancy.
-  Section with_var.
-    Import Straightline.expr.
-    Context {var : type -> Type} (dummy_arrow : forall s d, var (type.arrow s d)) (log2wordmax : Z)
-            (constant_to_scalar : forall ident, Z -> option (@scalar var ident type.Z)).
-    Local Notation Z := (type.type_primitive type.Z).
+  Import Straightline.expr.
+  Section with_wordmax.
+    Context (log2wordmax : Z) (log2wordmax_pos : 1 < log2wordmax).
     Let wordmax := 2 ^ log2wordmax.
     Let half_bits := log2wordmax / 2.
     Let wordmax_half_bits := 2 ^ half_bits.
 
-    Inductive ident : type -> type -> Type :=
-    | add : ident (Z * Z) (Z * Z)
-    | addc : ident (Z * Z * Z) (Z * Z)
-    | mulll : ident (Z * Z) Z
-    | mullh : ident (Z * Z) Z
-    | mulhl : ident (Z * Z) Z
-    | mulhh : ident (Z * Z) Z
-    | sub : ident (Z * Z) (Z * Z)
-    | land : BinInt.Z -> ident Z Z
-    | shiftr : BinInt.Z -> ident Z Z
-    | shiftl : BinInt.Z -> ident Z Z
-    | rshi : BinInt.Z -> ident (Z * Z) Z
-    | selc : ident (Z * Z * Z) Z
-    | selm : ident (Z * Z * Z) Z
-    | sell : ident (Z * Z * Z) Z
-    | addm : ident (Z * Z * Z) Z
-    .
-    Definition dummy t : @expr var ident t := Scalar (dummy_scalar (dummy_arrow:=dummy_arrow) t).
+    Lemma wordmax_gt_2 : 2 < wordmax.
+    Proof.
+      clear - wordmax log2wordmax log2wordmax_pos. subst wordmax.
+      apply Z.le_lt_trans with (m:=2 ^ 1); [ reflexivity | ].
+      apply Z.pow_lt_mono_r; omega.
+    Qed.
 
-    Definition invert_lower' {t} (e : @scalar var ident t) :
-      option (@scalar var ident Z) :=
-      match e in scalar t return option (@scalar var ident Z) with
-      | Cast r (Land n x) =>
-        if (lower r =? 0) && (upper r =? (wordmax_half_bits - 1)) && (n =? 2^half_bits-1)
-        then Some x
-        else None
-      | _ => None
-      end.
+    Lemma wordmax_even : wordmax mod 2 = 0.
+    Proof.
+      replace 2 with (2 ^ 1) by reflexivity.
+      subst wordmax. apply Z.mod_same_pow; omega.
+    Qed.
 
-    Definition invert_upper' {t} (e : @scalar var ident t) :
-      option (@scalar var ident Z) :=
-      match e in scalar t return option (@scalar var ident Z) with
-      | Cast r (Shiftr n x) =>
-        if (lower r =? 0) && (upper r =? (wordmax_half_bits - 1)) && (n =? half_bits)
-        then Some x
-        else None
-      | _ => None
-      end.
+    Lemma wordmax_half_bits_pos : 0 < wordmax_half_bits.
+    Proof. subst wordmax_half_bits half_bits. Z.zero_bounds. Qed.
 
-    Definition invert_lower {t} (e : @scalar var ident t) :
-      option (@scalar var ident Z) :=
-      match e in scalar t return option (@scalar var ident Z) with
-      | Primitive type.Z x =>
-        match constant_to_scalar ident x with
-        | Some y => invert_lower' y
-        | None => None
-        end
-      | _ => invert_lower' e
-      end.
+    Lemma half_bits_squared : (wordmax_half_bits - 1) * (wordmax_half_bits - 1) <= wordmax - 1.
+    Proof.
+      pose proof wordmax_half_bits_pos.
+      subst wordmax_half_bits.
+      transitivity (2 ^ (half_bits + half_bits) - 2 * 2 ^ half_bits + 1).
+      { rewrite Z.pow_add_r by (subst half_bits; Z.zero_bounds).
+        autorewrite with push_Zmul; omega. }
+      { transitivity (wordmax - 2 * 2 ^ half_bits + 1); [ | lia].
+        subst wordmax.
+        apply Z.add_le_mono_r.
+        apply Z.sub_le_mono_r.
+        apply Z.pow_le_mono_r; [ omega | ].
+        rewrite Z.add_diag; subst half_bits.
+        apply BinInt.Z.mul_div_le; omega. }
+    Qed.
 
-    Definition invert_upper {t} (e : @scalar var ident t) :
-      option (@scalar var ident Z) :=
-      match e in scalar t return option (@scalar var ident Z) with
-      | Primitive type.Z x =>
-        match constant_to_scalar ident x with
-        | Some y => invert_upper' y
-        | None => None
-        end
-      | _ => invert_upper' e
-      end.
+    Section with_var.
+      Context {var : type -> Type} (dummy_arrow : forall s d, var (type.arrow s d))
+              (constant_to_scalar : Z -> option (@scalar var type.Z)).
+      Local Notation Z := (type.type_primitive type.Z).
 
-    Definition invert_sell {t} (e : @scalar var ident t) :
-      option (@scalar var ident Z * @scalar var ident Z *  @scalar var ident Z) :=
-      match e return _ with
-      | Pair _ Z (Pair Z Z x y) z =>
-        match x return option (@scalar var ident Z * @scalar var ident Z *  @scalar var ident Z) with
-        | Cast r (Land n x') =>
-          if (lower r =? 0) && (upper r =? 1) && (n =? 1)
-          then Some (x', y, z)
+      Inductive ident : type -> type -> Type :=
+      | add : ident (Z * Z) (Z * Z)
+      | addc : ident (Z * Z * Z) (Z * Z)
+      | mulll : ident (Z * Z) Z
+      | mullh : ident (Z * Z) Z
+      | mulhl : ident (Z * Z) Z
+      | mulhh : ident (Z * Z) Z
+      | sub : ident (Z * Z) (Z * Z)
+      (* | land : BinInt.Z -> ident Z Z *)
+      | shiftr : BinInt.Z -> ident Z Z
+      | shiftl : BinInt.Z -> ident Z Z
+      | rshi : BinInt.Z -> ident (Z * Z) Z
+      | selc : ident (Z * Z * Z) Z
+      | selm : ident (Z * Z * Z) Z
+      | sell : ident (Z * Z * Z) Z
+      | addm : ident (Z * Z * Z) Z
+      .
+      Definition dummy t : @expr var ident t := Scalar (dummy_scalar (dummy_arrow:=dummy_arrow) t).
+
+      Definition invert_lower' {t} (e : @scalar var t) :
+        option (@scalar var Z) :=
+        match e in scalar t return option (@scalar var Z) with
+        | Cast r (Land n x) =>
+          if (lower r =? 0) && (upper r =? (wordmax_half_bits - 1)) && (n =? 2^half_bits-1)
+          then Some x
           else None
-        | _ => (@None _)
-        end
-      | _ => None
-      end.
+        | _ => None
+        end.
 
-    Definition invert_selm {t} (e : @scalar var ident t) :
-      option (@scalar var ident Z * @scalar var ident Z *  @scalar var ident Z) :=
-      match e return _ with
-      | Pair _ Z (Pair Z Z x y) z =>
-        match x return option (@scalar var ident Z * @scalar var ident Z *  @scalar var ident Z) with
-        | Cast r (CC_m n x') =>
-          if (lower r =? 0) && (upper r =? 1) && (n =? wordmax)
-          then Some (x', y, z)
+      Definition invert_upper' {t} (e : @scalar var t) :
+        option (@scalar var Z) :=
+        match e in scalar t return option (@scalar var Z) with
+        | Cast r (Shiftr n x) =>
+          if (lower r =? 0) && (upper r =? (wordmax_half_bits - 1)) && (n =? half_bits)
+          then Some x
           else None
-        | _ => (@None _)
-        end
-      | _ => None
-      end.
+        | _ => None
+        end.
 
-    Definition of_straightline_ident {s d} (idc : ident.ident s d)
-      : forall t, range_type d -> @scalar var ident s -> (var d -> @expr var ident t) -> @expr var ident t :=
-      match idc in ident.ident s d return forall t, range_type d -> scalar s -> (var d -> @expr var ident t) -> @expr var ident t with
-      | ident.Z.add_get_carry_concrete w =>
-        fun t r x f =>
-          if w =? wordmax
-          then LetInAppIdentZZ r add x f
-          else dummy _
-      | ident.Z.add_with_get_carry_concrete w =>
-        fun t r x f =>
-          if w =? wordmax
-          then LetInAppIdentZZ r addc x f
-          else dummy _
-      | ident.Z.sub_get_borrow_concrete w =>
-        fun t r x f =>
-          if w =? wordmax
-          then LetInAppIdentZZ r sub x f
-          else dummy _
-      | ident.Z.land n => fun _ r => LetInAppIdentZ r (land n)
-      | ident.Z.shiftr n => fun _ r => LetInAppIdentZ r (shiftr n)
-      | ident.Z.shiftl n => fun _ r => LetInAppIdentZ r (shiftl n)
-      | ident.Z.rshi_concrete w n =>
-        fun _ r x f =>
-          if w =? wordmax
-          then LetInAppIdentZ r (rshi n) x f
-          else dummy _
-      | ident.Z.zselect =>
-        fun t r x f =>
-          match invert_selm x with
-          | Some (x, y, z) => LetInAppIdentZ r selm (Pair (Pair x y) z) f
-          | None => match invert_sell x with
-                    | Some (x, y, z) => LetInAppIdentZ r sell (Pair (Pair x y) z) f
-                    | None => LetInAppIdentZ r selc x f
-                    end
+      Definition invert_lower {t} (e : @scalar var t) :
+        option (@scalar var Z) :=
+        match e in scalar t return option (@scalar var Z) with
+        | Primitive type.Z x =>
+          match constant_to_scalar x with
+          | Some y => invert_lower' y
+          | None => None
           end
-      | ident.Z.add_modulo => fun _ r => LetInAppIdentZ r addm
-      | ident.Z.mul =>
-        fun t r x f =>
-          match x return expr t with
-          | Pair _ _ x0 x1 =>
-            match invert_lower x0, invert_lower x1 with
-            | Some y0, Some y1 => LetInAppIdentZ r mulll (Pair y0 y1) f
-            | Some y0, None =>
-              match invert_upper x1 with
-              | Some y1 => LetInAppIdentZ r mullh (Pair y0 y1) f
-              | None => dummy _
-              end
-            | None, Some y1 =>
-              match invert_upper x0 with
-              | Some y0 => LetInAppIdentZ r mulhl (Pair y0 y1) f
-              | None => dummy _
-              end
-            | None, None =>
-              match invert_upper x0, invert_upper x1 with
-              | Some y0, Some y1 => LetInAppIdentZ r mulhh (Pair y0 y1) f
-              | _,_ => dummy _
-              end
+        | _ => invert_lower' e
+        end.
+
+      Definition invert_upper {t} (e : @scalar var t) :
+        option (@scalar var Z) :=
+        match e in scalar t return option (@scalar var Z) with
+        | Primitive type.Z x =>
+          match constant_to_scalar x with
+          | Some y => invert_upper' y
+          | None => None
+          end
+        | _ => invert_upper' e
+        end.
+
+      Definition invert_sell {t} (e : @scalar var t) :
+        option (@scalar var Z * @scalar var Z *  @scalar var Z) :=
+        match e return _ with
+        | Pair _ Z (Pair Z Z x y) z =>
+          match x return option (@scalar var Z * @scalar var Z *  @scalar var Z) with
+          | Cast r (Land n x') =>
+            if (lower r =? 0) && (upper r =? 1) && (n =? 1)
+            then Some (x', y, z)
+            else None
+          | _ => (@None _)
+          end
+        | _ => None
+        end.
+
+      Definition invert_selm {t} (e : @scalar var t) :
+        option (@scalar var Z * @scalar var Z *  @scalar var Z) :=
+        match e return _ with
+        | Pair _ Z (Pair Z Z x y) z =>
+          match x return option (@scalar var Z * @scalar var Z *  @scalar var Z) with
+          | Cast r (CC_m n x') =>
+            if (lower r =? 0) && (upper r =? 1) && (n =? wordmax)
+            then Some (x', y, z)
+            else None
+          | _ => (@None _)
+          end
+        | _ => None
+        end.
+
+      Definition of_straightline_ident {s d} (idc : ident.ident s d)
+        : forall t, range_type d -> @scalar var s -> (var d -> @expr var ident t) -> @expr var ident t :=
+        match idc in ident.ident s d return forall t, range_type d -> scalar s -> (var d -> @expr var ident t) -> @expr var ident t with
+        | ident.Z.add_get_carry_concrete w =>
+          fun t r x f =>
+            if w =? wordmax
+            then LetInAppIdentZZ r add x f
+            else dummy _
+        | ident.Z.add_with_get_carry_concrete w =>
+          fun t r x f =>
+            if w =? wordmax
+            then LetInAppIdentZZ r addc x f
+            else dummy _
+        | ident.Z.sub_get_borrow_concrete w =>
+          fun t r x f =>
+            if w =? wordmax
+            then LetInAppIdentZZ r sub x f
+            else dummy _
+        (* | ident.Z.land n => fun _ r => LetInAppIdentZ r (land n) *)
+        | ident.Z.shiftr n => fun _ r => LetInAppIdentZ r (shiftr n)
+        | ident.Z.shiftl n => fun _ r => LetInAppIdentZ r (shiftl n)
+        | ident.Z.rshi_concrete w n =>
+          fun _ r x f =>
+            if w =? wordmax
+            then LetInAppIdentZ r (rshi n) x f
+            else dummy _
+        | ident.Z.zselect =>
+          fun t r x f =>
+            match invert_selm x with
+            | Some (x, y, z) => LetInAppIdentZ r selm (Pair (Pair x y) z) f
+            | None => match invert_sell x with
+                      | Some (x, y, z) => LetInAppIdentZ r sell (Pair (Pair x y) z) f
+                      | None => LetInAppIdentZ r selc x f
+                      end
             end
-          | _ => dummy _
+        | ident.Z.add_modulo => fun _ r => LetInAppIdentZ r addm
+        | ident.Z.mul =>
+          fun t r x f =>
+            match x return expr t with
+            | Pair _ _ x0 x1 =>
+              match invert_lower x0, invert_lower x1 with
+              | Some y0, Some y1 => LetInAppIdentZ r mulll (Pair y0 y1) f
+              | Some y0, None =>
+                match invert_upper x1 with
+                | Some y1 => LetInAppIdentZ r mullh (Pair y0 y1) f
+                | None => dummy _
+                end
+              | None, Some y1 =>
+                match invert_upper x0 with
+                | Some y0 => LetInAppIdentZ r mulhl (Pair y0 y1) f
+                | None => dummy _
+                end
+              | None, None =>
+                match invert_upper x0, invert_upper x1 with
+                | Some y0, Some y1 => LetInAppIdentZ r mulhh (Pair y0 y1) f
+                | _,_ => dummy _
+                end
+              end
+            | _ => dummy _
+            end
+        | _ => fun t _ _ _ => dummy t
+        end.
+
+      Fixpoint of_straightline {t} (e : @expr var ident.ident t)
+        : @expr var ident t :=
+        match e with
+        | Scalar _ s => Scalar s 
+        | LetInAppIdentZ _ t r idc x f =>
+          of_straightline_ident idc t r x (fun y => of_straightline (f y))
+        | LetInAppIdentZZ _ t r idc x f =>
+          of_straightline_ident idc t r x (fun y => of_straightline (f y))
+        end.
+
+      Definition constant_to_scalar_single (const x : BinInt.Z) : option (@scalar var Z) :=
+        if x =? (BinInt.Z.shiftr const half_bits)
+        then Some (Cast {|lower := 0; upper:=wordmax_half_bits-1|} (Shiftr half_bits (Primitive (t:=type.Z) const)))
+        else if x =? (BinInt.Z.land const (wordmax_half_bits - 1))
+             then Some (Cast {|lower := 0; upper:=wordmax_half_bits-1|} (Land (wordmax_half_bits-1) (Primitive (t:=type.Z) const)))
+             else None.
+
+      Definition constant_to_scalar_gen (consts : list BinInt.Z) (x : BinInt.Z)
+        : option (Straightline.expr.scalar Z) :=
+        fold_right (fun c res => match res with
+                                 | Some s => Some s
+                                 | None => constant_to_scalar_single c x
+                                 end) None consts.
+    End with_var.
+
+    Section interp.
+      Local Notation low x := (Z.land x (wordmax_half_bits - 1)).
+      Local Notation high x := (x >> half_bits).
+
+      Definition interp_ident {s d} (idc : ident s d) : type.interp s -> type.interp d :=
+        match idc with
+        | add => fun x => Z.add_get_carry_full wordmax (fst x) (snd x)
+        | addc => fun x => Z.add_with_get_carry_full wordmax (fst (fst x)) (snd (fst x)) (snd x)
+        | mulll => fun x => low (fst x) * low (snd x)
+        | mullh => fun x => low (fst x) * high (snd x)
+        | mulhl => fun x => high (fst x) * low (snd x)
+        | mulhh => fun x => high (fst x) * high (snd x)
+        | sub => fun x => Z.sub_get_borrow_full wordmax (fst x) (snd x)
+       (* | land n => fun x => Z.land x n *) (* only allowed inside select/mul? *)
+        | shiftr n => fun x => Z.shiftr x n
+        | shiftl n => fun x => Z.shiftl x n
+        | rshi n => fun x => Z.rshi wordmax (fst x) (snd x) n
+        | selc => fun x => Z.zselect (fst (fst x)) (snd (fst x)) (snd x)
+        | selm => fun x => Z.zselect (Z.cc_m wordmax (fst (fst x))) (snd (fst x)) (snd x)
+        | sell => fun x => Z.zselect (Z.land (fst (fst x)) 1) (snd (fst x)) (snd x)
+        | addm => fun x => Z.add_modulo (fst (fst x)) (snd (fst x)) (snd x)
+        end.
+
+      Fixpoint interp {t} (e : @expr type.interp ident t) : type.interp t :=
+        match e with
+        | Scalar t s => interp_scalar s
+        | LetInAppIdentZ s d r idc x f =>
+          interp (f (interp_cast r (interp_ident idc (interp_scalar x))))
+        | LetInAppIdentZZ s d r idc x f =>
+          interp (f (interp_cast2 r (interp_ident idc (interp_scalar x))))
+        end.
+    End interp.
+
+    Section proofs.
+      Context (dummy_arrow : forall s d, type.interp (s -> d)%ctype)
+              (constant_to_scalar : Z -> option (@scalar type.interp type.Z)).
+
+      Local Notation word_range := (r[0~>wordmax-1])%zrange.
+      Local Notation half_word_range := (r[0~>wordmax_half_bits-1])%zrange.
+      Local Notation flag_range := (r[0~>1])%zrange.
+
+      Definition in_word_range (r : zrange) := is_tighter_than_bool r word_range = true.
+      Definition in_flag_range (r : zrange) := is_tighter_than_bool r flag_range = true.
+
+      Fixpoint get_range_var (t : type) : type.interp t -> range_type t :=
+        match t with
+        | type.type_primitive type.Z =>
+          fun x => {| lower := x; upper := x |}
+        | type.prod a b =>
+          fun x => (get_range_var a (fst x), get_range_var b (snd x))
+        | _ => fun _ => tt
+        end.
+      
+      Fixpoint get_range {t} (x : @scalar type.interp t) : range_type t :=
+        match x with
+        | Var t v => get_range_var t v
+        | TT => tt
+        | Nil _ => tt
+        | Pair _ _ x y => (get_range x, get_range y)
+        | Cast r _ => r
+        | Cast2 r _ => r
+        | Fst _ _ p => fst (get_range p)
+        | Snd _ _ p => snd (get_range p)
+        | Shiftr n x => ZRange.map (fun y => Z.shiftr y n) (get_range x)
+        | Shiftl n x => ZRange.map (fun y => Z.shiftl y n) (get_range x)
+        | Land n x => r[0~>n]%zrange
+        | CC_m n x => ZRange.map (Z.cc_m n) (get_range x)
+        | Primitive type.Z x => {| lower := x; upper := x |}
+        | Primitive p x => tt
+        end.
+
+      Fixpoint has_range {t} : range_type t -> type.interp t -> Prop :=
+        match t with
+        | type.type_primitive type.Z =>
+          fun r x =>
+            lower r <= x <= upper r
+        | type.prod a b =>
+          fun r x =>
+            has_range (fst r) (fst x) /\ has_range (snd r) (snd x)
+        | _ => fun _ _ => True
+        end.
+
+      Inductive ok_scalar : forall {t}, @scalar type.interp t -> Prop :=
+      | sc_ok_var : forall t v, ok_scalar (Var t v)
+      | sc_ok_unit : ok_scalar TT
+      | sc_ok_nil : forall t, ok_scalar (Nil t)
+      | sc_ok_pair : forall A B x y,
+          @ok_scalar A x ->
+          @ok_scalar B y ->
+          ok_scalar (Pair x y)
+      | sc_ok_cast : forall r (x : scalar type.Z),
+          ok_scalar x ->
+          is_tighter_than_bool (get_range x) r = true ->
+          ok_scalar (Cast r x)
+      | sc_ok_cast2 : forall r (x : scalar (type.prod type.Z type.Z)),
+          ok_scalar x ->
+          is_tighter_than_bool (fst (get_range x)) (fst r) = true ->
+          is_tighter_than_bool (snd (get_range x)) (snd r) = true ->
+          ok_scalar (Cast2 r x)
+      | sc_ok_fst :
+          forall A B p, @ok_scalar (A * B) p -> ok_scalar (Fst p)
+      | sc_ok_snd :
+          forall A B p, @ok_scalar (A * B) p -> ok_scalar (Snd p)
+      | sc_ok_shiftr :
+          forall n x, 0 <= n -> ok_scalar x -> ok_scalar (Shiftr n x)
+      | sc_ok_shiftl :
+          forall n x, 0 <= n -> 0 <= lower (@get_range type.Z x) -> ok_scalar x -> ok_scalar (Shiftl n x)
+      | sc_ok_land :
+          forall n x, 0 <= n -> 0 <= lower (@get_range type.Z x) -> ok_scalar x -> ok_scalar (Land n x)
+      | sc_ok_cc_m :
+          forall x, ok_scalar x -> ok_scalar (CC_m wordmax x)
+      | sc_ok_prim : forall p x, ok_scalar (@Primitive _ p x)
+      .
+
+      Print ident.
+      Inductive ok_ident : forall s d, scalar s -> range_type d -> ident.ident s d -> Prop :=
+      | ok_add :
+          forall x : scalar (type.prod type.Z type.Z),
+            in_word_range (fst (get_range x)) ->
+            in_word_range (snd (get_range x)) ->
+            ok_ident _
+                     (type.prod type.Z type.Z)
+                     x
+                     (word_range, flag_range)
+                     (ident.Z.add_get_carry_concrete wordmax)
+      | ok_addc :
+          forall x : scalar (type.prod (type.prod type.Z type.Z) type.Z),
+            in_flag_range (fst (fst (get_range x))) ->
+            in_word_range (snd (fst (get_range x))) ->
+            in_word_range (snd (get_range x)) ->
+            ok_ident _
+                     (type.prod type.Z type.Z)
+                     x
+                     (word_range, flag_range)
+                     (ident.Z.add_with_get_carry_concrete wordmax)
+      | ok_sub :
+          forall x : scalar (type.prod type.Z type.Z),
+            in_word_range (fst (get_range x)) ->
+            in_word_range (snd (get_range x)) ->
+            ok_ident _
+                     (type.prod type.Z type.Z)
+                     x 
+                     (word_range, flag_range)
+                     (ident.Z.sub_get_borrow_concrete wordmax)
+     (* | ok_land :
+          forall (x : scalar type.Z) n,
+            in_word_range (get_range x) ->
+            0 <= n < wordmax ->
+            ok_ident type.Z type.Z x (ZRange.map (fun y => Z.land y n) (get_range x)) (ident.Z.land n)*)
+      | ok_shiftr :
+          forall (x : scalar type.Z) n,
+            in_word_range (get_range x) ->
+            0 <= n <= log2wordmax ->
+            ok_ident type.Z type.Z x (ZRange.map (fun y => Z.shiftr y n) (get_range x)) (ident.Z.shiftr n)
+      | ok_shiftl :
+          forall (x : scalar type.Z) n,
+            in_word_range (get_range x) ->
+            0 <= n < log2wordmax - Z.log2_up (upper (get_range x)) ->
+            ok_ident type.Z type.Z x word_range (ident.Z.shiftl n)
+      | ok_rshi :
+          forall (x : scalar (type.prod type.Z type.Z)) n,
+            in_word_range (fst (get_range x)) ->
+            in_word_range (snd (get_range x)) ->
+            0 <= n < 2 * log2wordmax ->
+            ok_ident (type.prod type.Z type.Z) type.Z x word_range (ident.Z.rshi_concrete wordmax n)
+      | ok_selc :
+          forall (x : scalar (type.prod type.Z type.Z)) (y z : scalar type.Z),
+            in_flag_range (snd (get_range x)) ->
+            in_word_range (get_range y) ->
+            in_word_range (get_range z) ->
+            ok_ident _ 
+                     type.Z
+                     (Pair (Pair (Snd x) y) z)
+                     word_range
+                     ident.Z.zselect
+      | ok_selm :
+          forall x y z : scalar type.Z,
+            in_word_range (get_range x) ->
+            in_word_range (get_range y) ->
+            in_word_range (get_range z) ->
+            ok_ident _ 
+                     type.Z
+                     (Pair (Pair (Cast flag_range (CC_m wordmax x)) y) z)
+                     word_range
+                     ident.Z.zselect
+      | ok_sell :
+          forall x y z : scalar type.Z,
+            in_word_range (get_range x) ->
+            in_word_range (get_range y) ->
+            in_word_range (get_range z) ->
+            ok_ident _ 
+                     type.Z
+                     (Pair (Pair (Cast flag_range (Land 1 x)) y) z)
+                     word_range
+                     ident.Z.zselect
+      | ok_addm :
+          forall (x : scalar (type.prod (type.prod type.Z type.Z) type.Z)),
+            in_word_range (fst (fst (get_range x))) ->
+            in_word_range (snd (fst (get_range x))) ->
+            in_word_range (snd (get_range x)) ->
+            upper (fst (fst (get_range x))) + upper (snd (fst (get_range x))) - lower (snd (get_range x)) < wordmax ->
+            ok_ident _
+                     type.Z
+                     x 
+                     word_range
+                     ident.Z.add_modulo
+      | ok_mulll :
+          forall x y : scalar type.Z,
+            in_word_range (get_range x) ->
+            in_word_range (get_range y) ->
+            ok_ident (type.prod type.Z type.Z)
+                     type.Z
+                     (Pair
+                        (Cast half_word_range (Land (wordmax_half_bits - 1) x))
+                        (Cast half_word_range (Land (wordmax_half_bits - 1) y)))
+                     word_range
+                     ident.Z.mul
+      | ok_mullh :
+          forall x y : scalar type.Z,
+            in_word_range (get_range x) ->
+            in_word_range (get_range y) ->
+            ok_ident (type.prod type.Z type.Z)
+                     type.Z
+                     (Pair
+                        (Cast half_word_range (Land (wordmax_half_bits - 1) x))
+                        (Cast half_word_range (Shiftr half_bits y)))
+                     word_range
+                     ident.Z.mul
+      | ok_mulhl :
+          forall x y : scalar type.Z,
+            in_word_range (get_range x) ->
+            in_word_range (get_range y) ->
+            ok_ident (type.prod type.Z type.Z)
+                     type.Z
+                     (Pair
+                        (Cast half_word_range (Shiftr half_bits x))
+                        (Cast half_word_range (Land (wordmax_half_bits - 1) y)))
+                     word_range
+                     ident.Z.mul
+      | ok_mulhh :
+          forall x y : scalar type.Z,
+            in_word_range (get_range x) ->
+            in_word_range (get_range y) ->
+            ok_ident (type.prod type.Z type.Z)
+                     type.Z
+                     (Pair
+                        (Cast half_word_range (Shiftr half_bits x))
+                        (Cast half_word_range (Shiftr half_bits y)))
+                     word_range
+                     ident.Z.mul
+      .
+
+      Inductive ok_expr : forall {t}, @expr type.interp ident.ident t -> Prop :=
+      | ok_of_scalar : forall t s, @ok_expr t (Scalar s)
+      | ok_letin_z : forall s d r idc x f,
+          ok_ident _ type.Z x r idc ->
+          ok_scalar x ->
+          (forall y, has_range r y -> ok_expr (f y)) ->
+          ok_expr (@LetInAppIdentZ _ _ s d r idc x f)
+      | ok_letin_zz : forall s d r idc x f,
+          ok_ident _ (type.prod type.Z type.Z) x r idc ->
+          ok_scalar x ->
+          (forall y, has_range r y -> ok_expr (f y)) ->
+          ok_expr (@LetInAppIdentZZ _ _ s d r idc x f)
+      .
+
+      Ltac invert H :=
+        inversion H; subst;
+        repeat match goal with
+               | H : existT _ _ _ = existT _ _ _ |- _ => apply (Eqdep_dec.inj_pair2_eq_dec _ type.type_eq_dec) in H; subst
+               end.
+
+      Lemma has_range_get_range_var {t} (v : type.interp t) :
+        has_range (get_range_var _ v) v.
+      Proof.
+        induction t; cbn [get_range_var has_range fst snd]; auto.
+        destruct p; auto; cbn [upper lower]; omega.
+      Qed.
+
+      Lemma has_range_loosen r1 r2 (x : Z) :
+        @has_range type.Z r1 x ->
+        is_tighter_than_bool r1 r2 = true ->
+        @has_range type.Z r2 x.
+      Proof.
+        cbv [is_tighter_than_bool has_range]; intros;
+          match goal with H : _ && _ = true |- _ => rewrite andb_true_iff in H; destruct H end;
+          Z.ltb_to_lt; omega.
+      Qed.
+
+      Lemma interp_cast_noop x r :
+        @has_range type.Z r x ->
+        interp_cast r x = x.
+      Proof.
+        cbv [has_range interp_cast ident.cast]; intros.
+        break_match;
+          try match goal with H : _ && _ = true |- _ => rewrite andb_true_iff in H; destruct H end;
+          try match goal with H : _ && _ = false |- _ => rewrite andb_false_iff in H; destruct H end;
+          Z.ltb_to_lt; omega.
+      Qed.
+
+      Lemma interp_cast2_noop x r :
+        @has_range (type.prod type.Z type.Z) r x ->
+        interp_cast2 r x = x.
+      Proof.
+        cbv [has_range interp_cast2 interp_cast ident.cast]; intros.
+        break_match; destruct x;
+          repeat match goal with H : _ && _ = true |- _ => rewrite andb_true_iff in H; destruct H end;
+          repeat match goal with H : _ && _ = false |- _ => rewrite andb_false_iff in H; destruct H end;
+          Z.ltb_to_lt; try omega; reflexivity.
+      Qed.
+
+      Lemma has_range_shiftr n (x : scalar type.Z) :
+        0 <= n ->
+        has_range (get_range x) (interp_scalar x) ->
+        @has_range type.Z (ZRange.map (fun y : Z => y >> n) (get_range x)) (interp_scalar x >> n).
+      Proof. cbv [has_range]; intros; cbn. auto using Z.shiftr_le with omega. Qed.
+      Hint Resolve has_range_shiftr : has_range.
+
+      Lemma has_range_shiftl n r x :
+        0 <= n -> 0 <= lower r ->
+        @has_range type.Z r x ->
+        @has_range type.Z (ZRange.map (fun y : Z => y << n) r) (x << n).
+      Proof. cbv [has_range]; intros; cbn. auto using Z.shiftl_le_mono with omega. Qed.
+      Hint Resolve has_range_shiftl : has_range.
+
+      Lemma has_range_land n (x : scalar type.Z) :
+        0 <= n -> 0 <= lower (get_range x) ->
+        has_range (get_range x) (interp_scalar x) ->
+        @has_range type.Z (r[0~>n])%zrange (Z.land (interp_scalar x) n).
+      Proof.
+        cbv [has_range]; intros; cbn.
+        split; [ apply Z.land_nonneg | apply Z.land_upper_bound_r ]; omega.
+      Qed.
+      Hint Resolve has_range_land : has_range.
+
+      Lemma has_range_interp_scalar {t} (x : scalar t) :
+        ok_scalar x ->
+        has_range (get_range x) (interp_scalar x).
+      Proof.
+        induction 1; cbn [interp_scalar get_range];
+          auto with has_range;
+          try solve [try inversion IHok_scalar; cbn [has_range];
+                     auto using has_range_get_range_var]; [ | | | ].
+        { rewrite interp_cast_noop by eauto using has_range_loosen.
+          eapply has_range_loosen; eauto. }
+        { inversion IHok_scalar.
+          rewrite interp_cast2_noop;
+            cbn [has_range]; split; eapply has_range_loosen; eauto. }
+        { cbn. cbv [has_range] in *.
+          pose proof wordmax_gt_2.
+          rewrite !Z.cc_m_eq by omega.
+          split; apply Z.div_le_mono; Z.zero_bounds; omega. }
+        { destruct p; cbn [has_range upper lower]; auto; omega. }
+      Qed.
+      Hint Resolve has_range_interp_scalar : has_range.
+
+      Lemma has_word_range_interp_scalar (x : scalar type.Z) :
+        ok_scalar x ->
+        in_word_range (get_range x) ->
+        @has_range type.Z word_range (interp_scalar x).
+      Proof. eauto using has_range_loosen, has_range_interp_scalar. Qed.
+
+      Lemma in_word_range_nonneg r : in_word_range r -> 0 <= lower r.
+      Proof.
+        cbv [in_word_range is_tighter_than_bool].
+        rewrite andb_true_iff; intuition.
+      Qed.
+
+      Lemma in_word_range_upper_nonneg r x : @has_range type.Z r x -> in_word_range r -> 0 <= upper r.
+      Proof.
+        cbv [in_word_range is_tighter_than_bool]; cbn.
+        rewrite andb_true_iff; intuition.
+        Z.ltb_to_lt. omega.
+      Qed.
+
+      Lemma has_word_range_shiftl n r x :
+        0 <= n < log2wordmax - Z.log2_up (upper r) ->
+        @has_range type.Z r x ->
+        in_word_range r ->
+        @has_range type.Z word_range (x << n).
+      Proof.
+        intros.
+        eapply has_range_loosen;
+          [ apply has_range_shiftl; eauto using in_word_range_nonneg with has_range; omega | ].
+        cbv [is_tighter_than_bool]. cbn.
+        apply andb_true_iff; split; apply Z.leb_le;
+          [ apply Z.shiftl_nonneg; solve [auto using in_word_range_nonneg] | ].
+        rewrite Z.shiftl_mul_pow2 by omega.
+        destruct (dec (upper r = 0));
+          [ match goal with H : _ = 0 |- _ => rewrite H end; pose proof wordmax_gt_2; lia | ].
+        match goal with |- ?a * ?b <= _ =>
+                        transitivity (2 ^ (Z.log2_up a) * b) end.
+        { apply Z.mul_le_mono_nonneg_r; auto with zarith; [ ].
+          apply Z.log2_log2_up_spec.
+          apply Z.le_neq; eauto using in_word_range_upper_nonneg with has_range. }
+        { rewrite <-Z.pow_add_r by auto with zarith.
+          assert (2 ^ (Z.log2_up (upper r) + n) < 2 ^ log2wordmax)
+            by (apply Z.pow_lt_mono_r; omega).
+          replace wordmax with (2 ^ log2wordmax) by reflexivity.
+          omega. }
+      Qed.
+
+      Lemma has_word_range_rshi n x y :
+        0 <= n ->
+        @has_range type.Z word_range (Z.rshi wordmax x y n).
+      Proof.
+        pose proof wordmax_gt_2.
+        intros; rewrite Z.rshi_correct by omega.
+        match goal with |- context [?x mod ?m] => pose proof (Z.mod_pos_bound x m ltac:(omega)) end.
+        cbn [has_range lower upper]; lia.
+      Qed.
+
+      Lemma in_word_range_spec r :
+        0 <= lower r -> upper r <= wordmax - 1 ->
+        in_word_range r.
+      Proof.
+        intros; cbv [in_word_range is_tighter_than_bool].
+        apply andb_true_iff.
+        split; apply Z.leb_le; cbn [upper lower]; omega.
+      Qed.
+
+      Ltac destruct_scalar :=
+        match goal with
+        | x : scalar (type.prod (type.prod _ _) _) |- _ =>
+          match goal with |- context [interp_scalar x] =>
+            destruct (interp_scalar x) as [ [? ?] ?];
+            destruct (get_range x) as [ [? ?] ?]
           end
-      | _ => fun t _ _ _ => dummy t
-      end.
+        | x : scalar (type.prod _ _) |- _ =>
+          match goal with |- context [interp_scalar x] =>
+            destruct (interp_scalar x) as [? ?]; destruct (get_range x) as [? ?]
+          end
+        end.
 
-    Fixpoint of_straightline_scalar {t} (s : @scalar var ident.ident t)
-      : @scalar var ident t :=
-      match s with
-      | Var _ v => Var _ v
-      | TT => TT
-      | Nil _ => Nil _
-      | Pair _ _ x y => Pair (of_straightline_scalar x) (of_straightline_scalar y)
-      | Cast r x => Cast r (of_straightline_scalar x)
-      | Cast2 r x => Cast2 r (of_straightline_scalar x)
-      | Fst _ _ x => Fst (of_straightline_scalar x)
-      | Snd _ _ x => Snd (of_straightline_scalar x)
-      | Shiftr n x => Shiftr n (of_straightline_scalar x)
-      | Shiftl n x => Shiftl n (of_straightline_scalar x)
-      | Land n x => Land n (of_straightline_scalar x)
-      | CC_m n x => CC_m n (of_straightline_scalar x)
-      | Primitive _ x => Primitive x
-      end.
+      Lemma ident_interp_has_range s d x r idc:
+        ok_scalar x ->
+        ok_ident s d x r idc ->
+        has_range r (ident.interp idc (interp_scalar x)).
+      Proof.
+        intro.
+        pose proof (has_range_interp_scalar x ltac:(assumption)).
+        pose proof wordmax_gt_2.
+        induction 1; cbn [ident.interp ident.gen_interp]; intros; try destruct_scalar;
+          repeat match goal with
+                 | H : _ && _ = true |- _ => rewrite andb_true_iff in H; destruct H; Z.ltb_to_lt
+                 |  H : _ /\ _ |- _ => destruct H
+                 | _ => progress subst
+                 | _ => progress (cbv [in_word_range in_flag_range is_tighter_than_bool] in * )
+                 | _ => progress (cbn [interp_scalar get_range has_range upper lower fst snd] in * )
+                 end.
+        {
+          autorewrite with to_div_mod.
+          match goal with |- context[?x mod ?m] => pose proof (Z.mod_pos_bound x m ltac:(omega)) end.
+          rewrite Z.div_between_0_if by omega.
+          split; break_match; lia. }
+        {
+          autorewrite with to_div_mod.
+          match goal with |- context[?x mod ?m] => pose proof (Z.mod_pos_bound x m ltac:(omega)) end.
+          rewrite Z.div_between_0_if by omega.
+          split; break_match; lia. }
+        {
+          autorewrite with to_div_mod.
+          match goal with |- context[?x mod ?m] => pose proof (Z.mod_pos_bound x m ltac:(omega)) end.
+          rewrite Z.div_sub_small by omega.
+          split; break_match; lia. }
+        { apply has_range_shiftr; cbn [has_range]; omega. }
+        { eapply has_word_range_shiftl; eauto using in_word_range_spec with has_range omega. }
+        { apply has_word_range_rshi; omega. }
+        { rewrite Z.zselect_correct. break_match; omega. }
+        { cbn [interp_scalar fst snd get_range] in *.
+          rewrite Z.zselect_correct. break_match; omega. }
+        { cbn [interp_scalar fst snd get_range] in *.
+          rewrite Z.zselect_correct. break_match; omega. }
+        { rewrite Z.add_modulo_correct.
+          break_match; Z.ltb_to_lt; omega. }
+        { cbn [interp_scalar fst snd get_range upper lower] in *.
+          pose proof half_bits_squared. nia. }
+        { cbn [interp_scalar fst snd get_range upper lower] in *.
+          pose proof half_bits_squared. nia. }
+        { cbn [interp_scalar fst snd get_range upper lower] in *.
+          pose proof half_bits_squared. nia. }
+        { cbn [interp_scalar fst snd get_range upper lower] in *.
+          pose proof half_bits_squared. nia. }
+      Qed.
 
-    Fixpoint of_straightline {t} (e : @expr var ident.ident t)
-      : @expr var ident t :=
-      match e with
-      | Scalar _ s => Scalar (of_straightline_scalar s)
-      | LetInAppIdentZ _ t r idc x f =>
-        of_straightline_ident idc t r (of_straightline_scalar x) (fun y => of_straightline (f y))
-      | LetInAppIdentZZ _ t r idc x f =>
-        of_straightline_ident idc t r (of_straightline_scalar x) (fun y => of_straightline (f y))
-      end.
+      Ltac extract_ok_scalar' level x :=
+        match goal with
+        | H : ok_scalar (Pair (Pair (?f (?g x)) _) _) |- _ =>
+          match (eval compute in (4 <=? level)) with
+          | true => invert H; extract_ok_scalar' 3 x
+          | _ => fail
+          end
+        | H : ok_scalar (Pair (?f (?g x)) _) |- _ =>
+          match (eval compute in (3 <=? level)) with
+          | true => invert H; extract_ok_scalar' 2 x
+          | _ => fail
+          end
+        | H : ok_scalar (?f (?g x)) |- _ =>
+          match (eval compute in (2 <=? level)) with
+          | true => invert H; extract_ok_scalar' 1 x
+          | _ => fail
+          end
+        | H : ok_scalar (?g x) |- _ => invert H
+        end.
+      
 
-    Definition constant_to_scalar_single ident (const x : BinInt.Z) : option (@Straightline.expr.scalar var ident Z) :=
-      if x =? (BinInt.Z.shiftr const half_bits)
-      then Some (Cast {|lower := 0; upper:=wordmax_half_bits-1|} (Shiftr half_bits (Primitive (t:=type.Z) const)))
-      else if x =? (BinInt.Z.land const (wordmax_half_bits - 1))
-           then Some (Cast {|lower := 0; upper:=wordmax_half_bits-1|} (Land (wordmax_half_bits-1) (Primitive (t:=type.Z) const)))
-           else None.
+      Ltac extract_ok_scalar :=
+        match goal with |- ok_scalar ?x => extract_ok_scalar' 4 x; assumption end.
 
-    Definition constant_to_scalar_gen (consts : list BinInt.Z) ident (x : BinInt.Z)
-      : option (Straightline.expr.scalar Z) :=
-      fold_right (fun c res => match res with
-                               | Some s => Some s
-                               | None => constant_to_scalar_single ident c x
-                               end) None consts.
-  End with_var.
+      Lemma has_flag_range_cc_m r x :
+        @has_range type.Z r x ->
+        in_word_range r ->
+        @has_range type.Z flag_range (Z.cc_m wordmax x).
+      Proof.
+        cbv [has_range in_word_range is_tighter_than_bool].
+        cbn [upper lower]; rewrite andb_true_iff; intros.
+        match goal with H : _ /\ _ |- _ => destruct H; Z.ltb_to_lt end.
+        pose proof wordmax_gt_2. pose proof wordmax_even.
+        pose proof (Z.cc_m_small wordmax x). omega.
+      Qed.
+
+      Lemma has_flag_range_cc_m' (x : scalar type.Z) :
+        ok_scalar x ->
+        in_word_range (get_range x) ->
+        @has_range type.Z flag_range (Z.cc_m wordmax (interp_scalar x)).
+      Proof. eauto using has_flag_range_cc_m with has_range. Qed.
+
+      Lemma has_flag_range_land r x :
+        @has_range type.Z r x ->
+        in_word_range r ->
+        @has_range type.Z flag_range (Z.land x 1).
+      Proof.
+        cbv [has_range in_word_range is_tighter_than_bool].
+        cbn [upper lower]; rewrite andb_true_iff; intuition; Z.ltb_to_lt.
+        { apply Z.land_nonneg. left; omega. }
+        { apply Z.land_upper_bound_r; omega. }
+      Qed.
+
+      Lemma has_flag_range_land' (x : scalar type.Z) :
+        ok_scalar x ->
+        in_word_range (get_range x) ->
+        @has_range type.Z flag_range (Z.land (interp_scalar x) 1).
+      Proof. eauto using has_flag_range_land with has_range. Qed.
+
+      Ltac rewrite_cast_noop_in_mul :=
+        repeat match goal with
+               | _ => rewrite interp_cast_noop with (r:=half_word_range) in *
+                   by (eapply has_range_loosen; auto using has_range_land, has_range_interp_scalar)
+               | _ => rewrite interp_cast_noop with (r:=half_word_range) in *
+                   by (eapply has_range_loosen; try apply has_range_shiftr; auto using has_range_interp_scalar;
+                       cbn [ZRange.map get_range] in *; auto)
+               | _ => rewrite interp_cast_noop by assumption
+               end.
+
+      Lemma of_straightline_ident_correct s d t x r (idc : ident.ident s d) g :
+        ok_ident s d x r idc ->
+        ok_scalar x ->
+        interp (of_straightline_ident dummy_arrow constant_to_scalar idc t r x g) =
+        interp (g (ident.interp idc (interp_scalar x))).
+      Proof.
+        intros.
+        pose proof wordmax_half_bits_pos.
+        pose proof (ident_interp_has_range _ _ x r idc ltac:(assumption) ltac:(assumption)).
+        induction H; cbn [of_straightline_ident ident.interp ident.gen_interp invert_selm invert_sell invert_upper invert_lower invert_upper' invert_lower'] in *; intros;
+          rewrite ?Z.eqb_refl; cbn [interp interp_ident andb]; try destruct_scalar;
+            repeat match goal with
+                   | _ => progress (cbn [fst snd interp_scalar] in * )
+                   | _ => progress break_match; [ ]
+                   | _ => rewrite interp_cast_noop with (r:=flag_range) in *
+                       by (apply has_flag_range_cc_m'; auto; extract_ok_scalar)
+                   | _ => rewrite interp_cast_noop with (r:=flag_range) in *
+                       by (apply has_flag_range_land'; auto; extract_ok_scalar)
+                   | H : _ = (_,_) |- _ => progress (inversion H; subst)
+                   | _ => rewrite interp_cast_noop by assumption
+                   | _ => rewrite interp_cast2_noop by assumption
+                   | _ => reflexivity
+                   end; [ | | | ]; (* leftover cases are the 4 kinds of multiplication *)
+              match goal with
+              | H1 : in_word_range (get_range ?x), H2 : in_word_range (get_range ?y) |- _ =>
+                extract_ok_scalar' 4 x; extract_ok_scalar' 4 y
+              end; rewrite_cast_noop_in_mul; reflexivity.
+      Qed.
+
+      Lemma of_straightline_correct {t} (e : expr t) :
+        ok_expr e ->
+        interp (of_straightline dummy_arrow constant_to_scalar e) = Straightline.expr.interp (interp_ident:=@ident.interp) e.
+      Proof.
+        induction 1; cbn [of_straightline]; intros;
+          repeat match goal with
+                 | _ => progress cbn [Straightline.expr.interp]
+                 | _ => rewrite of_straightline_ident_correct by auto
+                 | _ => rewrite interp_cast_noop by auto using ident_interp_has_range
+                 | _ => rewrite interp_cast2_noop by auto using ident_interp_has_range
+                 | H : forall y, has_range _ y -> interp _ = _ |- _ => rewrite H by auto using ident_interp_has_range
+                 | _ => reflexivity
+                 end.
+      Qed.
+    End proofs.
+  End with_wordmax.
 
   Definition of_Expr {s d} (log2wordmax : Z) (consts : list Z) (e : Expr (s -> d))
              (var : type -> Type) (x : var s) dummy_arrow : @Straightline.expr.expr var ident d :=
-    @of_straightline var dummy_arrow log2wordmax (@constant_to_scalar_gen var log2wordmax consts) _ (Straightline.of_Expr e var x dummy_arrow).
+    @of_straightline log2wordmax var dummy_arrow (@constant_to_scalar_gen log2wordmax var consts) _ (Straightline.of_Expr e var x dummy_arrow).
+
+  Lemma of_Expr_correct {s d} (log2wordmax : Z) (consts : list Z) (e : Expr (s -> d))
+        (e' : (type.interp s -> Uncurried.expr.expr d))
+        (x : type.interp s) dummy_arrow :
+    e type.interp = Abs e' ->
+    1 < log2wordmax ->
+    Straightline.expr.ok_expr (e' x) ->
+    ok_expr log2wordmax (of_uncurried (dummy_arrow:=dummy_arrow) (depth (fun _ : type => unit) (fun _ : type => tt) (e (fun _ : type => unit))) (e' x)) ->
+    (depth type.interp (@DefaultValue.type.default) (e' x) <= depth (fun _ : type => unit) (fun _ : type => tt) (e (fun _ : type => unit)))%nat ->
+    interp log2wordmax (of_Expr log2wordmax consts e type.interp x dummy_arrow) = @Uncurried.expr.interp _ (@ident.interp) _ (e type.interp) x.
+  Proof.
+    intro He'; intros; cbv [of_Expr Straightline.of_Expr].
+    rewrite He'; cbn [invert_Abs expr.interp].
+    rewrite of_straightline_correct by assumption.
+    erewrite Straightline.expr.of_uncurried_correct by eassumption.
+    reflexivity.
+  Qed.
+
   Module Notations.
     Import PrintingNotations.
     Import Straightline.expr.
